synctactic sugar for allModelElements and allModelLinks

fr.inria.atlanmod.coqtl.coq/core/Model.v
@@ -3,12 +3,17 @@ Set Implicit Arguments.
 (** * Model
   Each model is constructed by a list of {@code ModelElement} and {@ModelLink}. **)
 
-
 Class Model (ModelElement: Type) (ModelLink: Type) :=
   {
-    allModelElements : list ModelElement;
-    allModelLinks : list ModelLink;
+    modelElements : list ModelElement;
+    modelLinks : list ModelLink;
   }.
+
+Definition allModelElements {ModelElement: Type} {ModelLink: Type} (m: Model ModelElement ModelLink) : list ModelElement :=
+  (@modelElements _ _ m).
+
+Definition allModelLinks {ModelElement: Type} {ModelLink: Type} (m: Model ModelElement ModelLink) : list ModelLink :=
+  (@modelLinks _ _ m).
 
 (*
  allModelElements and allModelLinks are fields of record Model.
